SeprefUF.thy
@@ -34,6 +34,25 @@ begin
     using part_equiv_refl[of R x] by blast
 
 
+  definition per_supset_rel :: "('a per \<times> 'a per) set" where
+    "per_supset_rel
+      \<equiv> {(p1,p2). p1 \<inter> Domain p2 \<times> Domain p2 = p2 \<and> p1 \<inter> -(Domain p2 \<times> Domain p2) \<subseteq> Id}"
+
+  lemma per_supset_rel_dom: "(p1, p2) \<in> per_supset_rel \<Longrightarrow> Domain p1 \<supseteq> Domain p2"
+    by (auto simp: per_supset_rel_def)
+  
+  lemma per_supset_compare:
+    "(p1, p2) \<in> per_supset_rel \<Longrightarrow> x1\<in>Domain p2 \<Longrightarrow> x2\<in>Domain p2 \<Longrightarrow> per_compare p1 x1 x2 \<longleftrightarrow> per_compare p2 x1 x2"
+    by (auto simp: per_supset_rel_def)
+  
+  lemma per_supset_union: "(p1, p2) \<in> per_supset_rel \<Longrightarrow> x1\<in>Domain p2 \<Longrightarrow> x2\<in>Domain p2 \<Longrightarrow>
+    (per_union p1 x1 x2, per_union p2 x1 x2) \<in> per_supset_rel"
+    apply (clarsimp simp: per_supset_rel_def per_union_def Domain_unfold )
+    apply (intro subsetI conjI)
+    apply blast
+    apply force
+    done
+
 
   sepref_register per_init per_init' per_compare per_union
 
